src/lib/collections/Collections.Seqs_i.fsti
@@ -41,3 +41,6 @@ val slice_append_adds (#a:Type) (s:seq a) (i:nat) (j:nat{ i <= j /\ j <= length 
 
 val slice_seq_map_commute (#a #b:Type) (f:a -> b) (s:seq a) (i:nat) (j:nat{ i <= j /\ j <= length s }) :
   Lemma (slice (seq_map f s) i j == seq_map f (slice s i j))
+
+val append_distributes_seq_map (#a #b:Type) (f:a -> b) (s1 s2:seq a) : 
+  Lemma (seq_map f (s1 @| s2) == seq_map f s1 @| seq_map f s2)
