src/lib/util/Words.Seq_i.fsti
@@ -45,3 +45,6 @@ val nat_to_four_8_injective: unit ->
 val seq_to_four_LE_injective: unit ->
   Lemma (forall (#a:Type) (x x':seq4 a) . seq_to_four_LE x == seq_to_four_LE x' ==> x == x') 
 *)
+
+val append_distributes_seq_to_seq_four_LE (#a:Type) (x:seq a{length x % 4 == 0}) (y:seq a{length y % 4 == 0}) :
+  Lemma (seq_to_seq_four_LE (x @| y) == seq_to_seq_four_LE x @| seq_to_seq_four_LE y)
